Add parallel variant

src/extensions.v
@@ -1,4 +1,21 @@
 From DeleteTree Require Import delete_tree.
+From iris.heap_lang Require Import lib.par.
+
+Definition delete_tree_par: val :=
+  rec: "delete_tree" "x" :=
+    match: !"x" with
+      InjR "tree" =>
+      (* this time, delete in parallel *)
+      (let: "left" := Fst "tree" in
+       let: "right" := Snd "tree" in
+       ("delete_tree" "left" ||| "delete_tree" "right");;
+      (* then free the root pointer *)
+      Free "x")
+    | InjL <> =>
+      (* the way we've represented trees, even an empty tree is a pointer to a
+      None, so free that, too *)
+      Free "x"
+    end.
 
 (** Some extra functions that check that the tree definition makes sense (these
 allow you to construct one while delete_tree assumes it's possible) *)
@@ -19,7 +36,7 @@ Definition expand_right: val :=
 
 Section proof.
 
-Context `{!heapG Σ}.
+Context `{!heapG Σ} `{!spawnG Σ}.
 Implicit Types (t l r:loc).
 
 Theorem wp_mk_empty_tree :
@@ -67,6 +84,30 @@ Proof.
     iIntros "!> Hright".
     iApply "HΦ".
     iApply (tree_combine_some with "[$Hp $Hleft $Hright]").
+Qed.
+
+Theorem wp_delete_tree_par t :
+  {{{ tree t }}}
+    delete_tree_par #t
+  {{{ RET #(); emp }}}.
+Proof using All.
+  iLöb as "IH" forall (t).
+  iIntros (Φ) "Ht HΦ".
+  iDestruct (tree_unfold with "Ht") as "[Ht|Ht]"; wp_rec.
+  - wp_load; wp_pures.
+    wp_free.
+    iApply "HΦ"; auto.
+  - iDestruct "Ht" as (l r) "(Ht & Hl & Hr)".
+    wp_load; wp_pures.
+    wp_apply (wp_par (λ _, emp)%I (λ _, emp)%I with "[Hl] [Hr]").
+    + wp_apply ("IH" with "Hl"); iIntros "_"; wp_pures.
+      done.
+    + wp_apply ("IH" with "Hr"); iIntros "_"; wp_pures.
+      done.
+    + iIntros (??) "_ !>".
+      wp_pures.
+      wp_free.
+      iApply "HΦ"; auto.
 Qed.
 
 End proof.
